src/LockClientAll.v
@@ -1,0 +1,43 @@
+From sflib Require Import sflib.
+From Paco Require Import paco.
+Require Import Coq.Classes.RelationClasses Lia Program.
+Unset Universe Checking.
+From Fairness Require Export ITreeLib WFLib FairBeh NatStructs Mod pind Axioms OpenMod WMM Red IRed Wrapper WeakestAdequacy FairLock Concurrency LockClient FIFOSched SchedSim FIFOSched FIFOSchedSim ModAdequacy TicketLockW.
+From PromisingLib Require Import Loc Event.
+From PromisingSEQ Require Import TView.
+From Ordinal Require Export ClassicalHessenberg.
+Require Import Coq.Numbers.BinNums.
+
+Section ALL.
+  Definition client_spec := ClientSpec.mod.
+
+  Definition client_abstract_lock :=
+    OMod.close ClientImpl.omod (ModAdd WMem.mod FairLockW.mod).
+
+  Definition client_ticket_lock :=
+    OMod.close ClientImpl.omod (ModAdd WMem.mod TicketLock.mod ).
+
+  Theorem client_all
+    :
+    Adequacy.improves
+      (interp_all
+         (client_spec.(Mod.st_init))
+         (prog2ths client_spec [("thread1", tt↑); ("thread2", tt↑)]) 0)
+      (interp_all_fifo
+         (client_ticket_lock.(Mod.st_init))
+         (prog2ths client_ticket_lock [("thread1", tt↑); ("thread2", tt↑)]) 0)
+  .
+  Proof.
+    eapply Adequacy.improves_trans.
+    { eapply Adequacy.adequacy.
+      { instantiate (1:=nat_wf). econs. exact 0. }
+      { i. ss. eauto. }
+      { eapply ssim_implies_gsim; ss.
+        { instantiate (1:=id). ss. }
+        { eapply ssim_nondet_fifo; ss. ii. compute in H. des. inv H; des; ss. inv H1; ss. }
+      }
+    }
+    eapply Adequacy.improves_trans.
+    { eapply modsim_adequacy.
+  Admitted.
+End ALL.
